src/PlutusIR/Semantics/Static/Normalization/Normalizer.v
@@ -79,7 +79,7 @@ Theorem normalizer__well_kinded Δ T Tn :
 Proof.
   unfold normalizer.
   move: eq_refl.
-  case: {2 3}(kind_check Δ T) => // a e H. (* TODO: I don't understand (all of) this ssreflect stuff, see https://stackoverflow.com/questions/47345174/using-destruct-on-pattern-match-expression-with-convoy-pattern*)
+  case: {2 3}(kind_check Δ T) => // a e H.
   inversion H.
   intros.
   exists a.
